woring on stlc

Stlc.v
@@ -134,3 +134,130 @@ Proof with auto.
   - intros H. induction H; simpl; try (rewrite <- beq_id_refl); 
     try (apply beq_id_false_iff in H; rewrite H); subst; auto.
 Qed.
+
+
+Reserved Notation "t1 '==>' t2" (at level 40).
+
+Inductive step : tm -> tm -> Prop :=
+  | ST_AppAbs : forall x T t12 v2,
+         value v2 ->
+         (tapp (tabs x T t12) v2) ==> [x:=v2]t12
+  | ST_App1 : forall t1 t1' t2,
+         t1 ==> t1' ->
+         tapp t1 t2 ==> tapp t1' t2
+  | ST_App2 : forall v1 t2 t2',
+         value v1 ->
+         t2 ==> t2' ->
+         tapp v1 t2 ==> tapp v1  t2'
+  | ST_IfTrue : forall t1 t2,
+      (tif ttrue t1 t2) ==> t1
+  | ST_IfFalse : forall t1 t2,
+      (tif tfalse t1 t2) ==> t2
+  | ST_If : forall t1 t1' t2 t3,
+      t1 ==> t1' ->
+      (tif t1 t2 t3) ==> (tif t1' t2 t3)
+
+where "t1 '==>' t2" := (step t1 t2).
+
+Hint Constructors step.
+
+Notation multistep := (multi step).
+Notation "t1 '==>*' t2" := (multistep t1 t2) (at level 40).
+
+Lemma step_example1 :
+  (tapp idBB idB) ==>* idB.
+Proof.
+  eapply multi_step.
+    apply ST_AppAbs.
+    apply v_abs.
+  simpl.
+  apply multi_refl. Qed.
+
+
+
+Lemma step_example5 :
+       (tapp (tapp idBBBB idBB) idB)
+  ==>* idB.
+Proof.
+  eapply multi_step.
+    apply ST_App1.
+    apply ST_AppAbs. constructor. simpl.
+  eapply multi_step.
+    apply ST_AppAbs. constructor. simpl.
+  constructor.
+Qed.
+
+Lemma step_example5_with_normalize :
+       (tapp (tapp idBBBB idBB) idB)
+  ==>* idB.
+Proof. normalize. Qed.
+
+Definition context := partial_map ty.
+
+Reserved Notation "Gamma '|-' t '\in' T" (at level 40).
+
+Inductive has_type : context -> tm -> ty -> Prop :=
+  | T_Var : forall Gamma x T,
+      Gamma x = Some T ->
+      Gamma |- tvar x \in T
+  | T_Abs : forall Gamma x T11 T12 t12,
+      update Gamma x T11 |- t12 \in T12 ->
+      Gamma |- tabs x T11 t12 \in TArrow T11 T12
+  | T_App : forall T11 T12 Gamma t1 t2,
+      Gamma |- t1 \in TArrow T11 T12 ->
+      Gamma |- t2 \in T11 ->
+      Gamma |- tapp t1 t2 \in T12
+  | T_True : forall Gamma,
+       Gamma |- ttrue \in TBool
+  | T_False : forall Gamma,
+       Gamma |- tfalse \in TBool
+  | T_If : forall t1 t2 t3 T Gamma,
+       Gamma |- t1 \in TBool ->
+       Gamma |- t2 \in T ->
+       Gamma |- t3 \in T ->
+       Gamma |- tif t1 t2 t3 \in T
+
+where "Gamma '|-' t '\in' T" := (has_type Gamma t T).
+
+Hint Constructors has_type.
+
+
+Example typing_example_1 :
+  empty |- tabs x TBool (tvar x) \in TArrow TBool TBool.
+Proof.
+  apply T_Abs. apply T_Var. reflexivity. Qed. 
+
+Example typing_example_3 :
+  exists T,
+    empty |-
+      (tabs x (TArrow TBool TBool)
+         (tabs y (TArrow TBool TBool)
+            (tabs z TBool
+               (tapp (tvar y) (tapp (tvar x) (tvar z)))))) \in
+      T.
+Proof with auto.
+  exists (TArrow (TArrow TBool TBool) (TArrow (TArrow TBool TBool) (TArrow TBool TBool))).
+  apply T_Abs.
+  apply T_Abs.
+  apply T_Abs.
+  eapply T_App. apply T_Var. reflexivity.
+  eapply T_App. apply T_Var. reflexivity.
+  apply T_Var. reflexivity.
+Qed.
+
+Example typing_nonexample_3 :
+  ~ (exists S, exists T,
+        empty |-
+          (tabs x S
+             (tapp (tvar x) (tvar x))) \in
+          T).
+Proof.
+  unfold not. intros. inversion H. clear H. inversion H0. clear H0.
+  inversion H. subst. clear H. inversion H5. subst. clear H5. inversion H2. subst. clear H2.
+  inversion H4. subst. clear H4. rewrite -> H2 in H1. inversion H1. clear H1. clear H2.
+  generalize dependent T12. induction T11.
+  + intros. inversion H0.
+  + intros. inversion H0. apply IHT11_1 with T11_2. auto.
+Qed.
+
+End STLC.
